いろいろ

TaPL/code/chapter3.v
@@ -10,14 +10,20 @@ Inductive value: term -> Prop :=
 
 Definition eg_1 : term := If (If True False False) False True.
 
-Inductive syntax: term -> term-> Prop :=
-  | EIfTrue: forall t2 t3, syntax (If True t2 t3) t2
-  | EIfFalse: forall t2 t3, syntax (If False t2 t3) t3
-  | EIf: forall t1 t1' t2 t3, (syntax t1 t1') -> (syntax (If t1 t2 t3) (If t1' t2 t3)).
+Inductive step: term -> term-> Prop :=
+  | EIfTrue: forall t2 t3, step (If True t2 t3) t2
+  | EIfFalse: forall t2 t3, step (If False t2 t3) t3
+  | EIf: forall t1 t1' t2 t3, (step t1 t1') -> (step (If t1 t2 t3) (If t1' t2 t3)).
 
 Inductive normal: term -> Prop :=
-| nexist: forall t, (forall t1, not (syntax t t1)) -> normal t.
+| nexist: forall t, (forall t1, not (step t t1)) -> normal t.
 
+Lemma If_one_step: forall t1 t2 t3, exists t, step (If t1 t2 t3) t.
+intros. generalize dependent t2. generalize dependent t3.
+induction t1. intros. exists t2. apply EIfTrue. intros. exists t3. apply EIfFalse.
+assert (exists t: term, step (If t1_1 t1_2 t1_3) t).
+apply IHt1_1. destruct H. intros.
+exists (If x t2 t3). apply EIf. apply H. Qed.
 
 Theorem thm3_5_7: forall t, value t -> normal t.
 intros. induction t. apply nexist. intros. unfold not. intros. inversion H0.
@@ -25,22 +31,59 @@ apply nexist. intros. unfold not. intros. inversion H0. inversion H.
 Qed.
 
 Theorem thm3_5_8: forall t, normal t -> value t. induction t.
-intros. apply v_true. intros. apply v_false. intros. induction t1. 
-inversion H. unfold not in H0. assert (syntax (If True t2 t3) t2). apply EIfTrue.
-apply H0 in H2. contradiction. inversion H. unfold not in H0.
-assert (syntax (If False t2 t3) t3). apply EIfFalse. apply H0 in H2. contradiction.
-assert (not (value (If t1_1 t1_2 t1_3))). unfold not. intros. inversion H0.
-assert (forall A B: Prop, (A->B) -> ((not B) -> (not A))). unfold not.
-intros. apply H1 in H3. apply H2 in H3. contradiction. apply H1 in IHt1.
-unfold not in IHt1. inversion H. unfold not in H2.
-inversion H.
-inversion H.
+intros. apply v_true. intros. apply v_false. intros. assert (exists x, step (If t1 t2 t3) x).
+apply If_one_step. destruct H0. assert (not (step (If t1 t2 t3) x)). inversion H. 
+apply H1. contradiction. Qed. 
 
-Theorem thm3_5_4: forall t1 t2 t3, (syntax t1 t2) -> (syntax t1 t3) -> t2=t3.
+Theorem thm3_5_4: forall t1 t2 t3, (step t1 t2) -> (step t1 t3) -> t2=t3.
 intros. generalize dependent t3.
 induction H. intros.
 inversion H0. reflexivity. subst. inversion H4.
 intros. inversion H0. subst. reflexivity. inversion H4.
 intros. inversion H0. subst. inversion H. subst. inversion H.  subst.
-apply IHsyntax in H5. subst. reflexivity. 
+apply IHstep in H5. subst. reflexivity. 
 Qed.  
+
+Inductive multistep: term->term->Prop:=
+  | Init: forall t1 t2, step t1 t2 -> multistep t1 t2
+  | Refl: forall t, multistep t t
+  | Trans: forall t1 t2 t3, multistep t1 t2 -> step t2 t3 -> multistep t1 t3.
+
+Lemma multitrans: forall t1 t2 t3, multistep t1 t2 -> multistep t2 t3 -> multistep t1 t3.
+intros. generalize dependent t1. induction H0. intros.
+apply Trans with (t2:=t1). exact H0. exact H. intros. exact H. intros. apply IHmultistep in H1.
+apply Trans with (t2 := t2). apply H1. apply H. Qed. 
+
+Lemma multi_true: forall t1 t2, value t1 -> multistep t1 t2 -> t2 = t1.
+intros. induction H0. inversion H. subst. inversion H0.
+subst. inversion H0. reflexivity. assert (value t1). apply H. apply IHmultistep in H. subst.
+inversion H2. subst. inversion H1. subst. inversion H1. Qed.
+
+
+Lemma multi_EIf: forall t1 t1' t2 t3, multistep t1 t1' -> multistep (If t1 t2 t3) (If t1' t2 t3).
+intros. generalize dependent t2. generalize dependent t3. induction H.
+intros. apply Init. apply EIf. exact H. intros. apply Refl.
+intros. apply Trans with (t2 := If t2 t4 t0). apply IHmultistep. apply EIf. apply H0. Qed.
+
+Lemma multi_IfTrue: forall t1 t2 t3, multistep t1 True -> multistep (If t1 t2 t3) t2.
+intros. assert (multistep (If t1 t2 t3) (If True t2 t3)). apply multi_EIf. exact H.
+apply Trans with (t2 := (If True t2 t3)). exact H0. apply EIfTrue. Qed.
+
+
+Lemma multi_IfFalse: forall t1 t2 t3, multistep t1 False -> multistep (If t1 t2 t3) t3.
+intros. assert (multistep (If t1 t2 t3) (If False t2 t3)). apply multi_EIf. exact H.
+apply Trans with (t2 := (If False t2 t3)). exact H0. apply EIfFalse. Qed.
+
+Theorem thm3_5_12: forall t, exists t1, multistep t t1 /\ normal t1.
+intros. induction t. exists True. split. apply Refl. apply thm3_5_7. apply v_true.
+exists False. split. apply Refl. apply thm3_5_7. apply v_false.
+destruct IHt1. destruct H. apply thm3_5_8 in H0. inversion H0. subst.
+apply multi_IfTrue with (t2 := t2) (t3 := t3) in H. destruct IHt2. destruct H1.
+assert ((multistep (If t1 t2 t3) t2)->(multistep t2 x)->multistep (If t1 t2 t3) x).
+apply multitrans. apply H3 in H. exists x. split. apply H. apply H2. apply H1.
+subst. apply multi_IfFalse with (t2:=t2) (t3:=t3) in H.  destruct IHt3. destruct H1.
+assert (multistep (If t1 t2 t3) t3 -> multistep t3 x -> multistep (If t1 t2 t3) x).
+apply multitrans. apply H3 in H. exists x. split. apply H. apply H2. apply H1. Qed.
+
+Theorem thm3_5_11: forall t u v, multistep t u -> multistep t v -> normal u -> normal v -> u = v.
+Admitted.
